Pass the routing_ipassmt generator a list of interfaces that have to be in the assignment — possibly empty.

thy/Iptables_Semantics/Primitive_Matchers/Routing_IpAssmt.thy
@@ -9,9 +9,9 @@ begin
 subsection\<open>Routing IP Assignment\<close>
 text\<open>Up to now, the definitions were all still on word intervals because those are much more convenient to work with.\<close>
 
-definition routing_ipassmt :: "'i::len routing_rule list \<Rightarrow> (iface \<times> ('i word \<times> nat) list) list"
+definition routing_ipassmt :: "'i::len routing_rule list \<Rightarrow> iface list \<Rightarrow> (iface \<times> ('i word \<times> nat) list) list"
   where
-  "routing_ipassmt rt \<equiv> map (apfst Iface \<circ> apsnd cidr_split) (routing_ipassmt_wi rt)"
+  "routing_ipassmt rt ifs \<equiv> map (apfst Iface \<circ> apsnd cidr_split) (routing_ipassmt_wi rt (map iface_sel ifs))"
 
 private lemma ipcidr_union_cidr_split[simp]: "ipcidr_union_set (set (cidr_split x)) = wordinterval_to_set x" 
   apply(subst cidr_split_prefix[symmetric])
@@ -22,16 +22,16 @@ private lemma map_of_map_Iface: "map_of (map (\<lambda>x. (Iface (fst x), f (snd
         map_option f ((map_of xs) ifce)"
   by (induct xs) (auto)
 
-lemma "routing_ipassmt_wi ([]::32 prefix_routing) = [(output_iface (routing_action (undefined :: 32 routing_rule)), WordInterval 0 0xFFFFFFFF)]"
+lemma "routing_ipassmt_wi ([]::32 prefix_routing) [] = [(output_iface (routing_action (undefined :: 32 routing_rule)), WordInterval 0 0xFFFFFFFF)]"
   by code_simp
 
 
 lemma routing_ipassmt: "
     valid_prefixes rt \<Longrightarrow>
     output_iface (routing_table_semantics rt (p_dst p)) = p_oiface p \<Longrightarrow>
-    \<exists>p_ips. map_of (routing_ipassmt rt) (Iface (p_oiface p)) = Some p_ips \<and> p_dst p \<in> ipcidr_union_set (set p_ips)"
+    \<exists>p_ips. map_of (routing_ipassmt rt ifs) (Iface (p_oiface p)) = Some p_ips \<and> p_dst p \<in> ipcidr_union_set (set p_ips)"
   apply(simp add: routing_ipassmt_def)
-  apply(drule routing_ipassmt_wi[where output_port="p_oiface p" and k="p_dst p"])
+  apply(drule routing_ipassmt_wi[where output_port="p_oiface p" and k="p_dst p" and ifs="map iface_sel ifs"])
   apply(simp)
   apply(elim exE, rename_tac ip_range)
   apply(rule_tac x="cidr_split ip_range" in exI)
@@ -39,22 +39,22 @@ lemma routing_ipassmt: "
   apply(simp add: comp_def)
   apply(simp add: map_of_map_Iface)
   apply(rule_tac x="ip_range" in exI)
-  apply(simp)
-  by (simp add: routing_ipassmt_wi_distinct)
+  apply(simp add: routing_ipassmt_wi_distinct)
+done
 
 lemma routing_ipassmt_ipassmt_sanity_disjoint: "valid_prefixes (rt::('i::len) prefix_routing) \<Longrightarrow>
-    ipassmt_sanity_disjoint (map_of (routing_ipassmt rt))"
+    ipassmt_sanity_disjoint (map_of (routing_ipassmt rt ifs))"
 unfolding ipassmt_sanity_disjoint_def routing_ipassmt_def comp_def
   apply(clarsimp)
   apply(drule map_of_SomeD)+
   apply(clarsimp split: iface.splits)
 using routing_ipassmt_wi_disjoint[where 'i = 'i] by meson
 
-lemma routing_ipassmt_distinct: "distinct (map fst (routing_ipassmt rtbl))"
+lemma routing_ipassmt_distinct: "distinct (map fst (routing_ipassmt rtbl ifs))"
   using routing_ipassmt_wi_distinct[of rtbl]
   unfolding routing_ipassmt_def
   apply(simp add: comp_def)
-  apply(subst distinct_map[where f = Iface and xs = "map fst (routing_ipassmt_wi rtbl)", simplified, unfolded comp_def])
+  apply(subst distinct_map[where f = Iface and xs = "map fst (routing_ipassmt_wi rtbl (map iface_sel ifs))", simplified, unfolded comp_def])
   apply(auto intro: inj_onI)
 done
   
